rocq-osiris/theories/program_logic/pure/judgements.v
@@ -5,62 +5,6 @@ From osiris.program_logic.pure Require Import wp.
 
 (** This file defines the judgements for pure computations. *)
 
-(* One justification for [Observe] appears in pure_rules.v, to generalize
-   [pure_bind] to more than just [@bind val val] *)
-
-(* -------------------------------------------------------------------------- *)
-
-(* Given an encodable value of type [A], it can be observed as a particular
-   value [V]. *)
-Class Observe A (EncA: Encode A) V : Type :=
-  { observe : A -> V }.
-
-Arguments Observe A {EncA} V.
-Arguments observe {_ _ _ _}.
-
-Global Instance observe_encode {A} `{Encode A}:
-  Observe A val :=
-  {| observe := encode |}.
-
-(* Useful for [pure (evals η _) φ ψ]. *)
-Global Instance observe_list {A} `{Encode A}:
-  Observe (list A) (list val) | 100 :=
-  {| observe := (map encode.encode) |}.
-
-(* NOTE : Do not declare an instance of [Observe val val], as it will
-   instantiate evars eagerly to this instance when it is not desired.
-   (Even if its weight is very high.) *)
-
-Notation "♯ x" := (observe x) (at level 5).
-
-(* -------------------------------------------------------------------------- *)
-
-Lemma solve_observe_nil A (Enc:Encode A) :
-  forall (xs : list A),
-    [] = xs →
-    nil = ♯xs.
-Proof. intros; subst; cbn; eauto. Qed.
-
-Lemma solve_observe_cons {A} {Enc: Encode A} :
-  forall (v : val) (a : A) tl vtl (x : list A),
-    a :: tl = x ->
-    v = # a ->
-    vtl = ♯ tl ->
-    v :: vtl = ♯ x.
-Proof.
-  induction tl; intros; subst; eauto.
-Qed.
-
-Global Hint Extern 0 (_ :: _ = ♯ _) =>
-  simple eapply solve_observe_cons : encode.
-Global Hint Extern 100 ([] = ♯ _) =>
-  simple eapply solve_observe_nil: encode.
-
-(* -------------------------------------------------------------------------- *)
-
-Definition returns {A V} `{Observe A V} (φ : A -> Prop):=
-  λ (v : V), ∃ a, v = observe a ∧ φ a.
-
 (* -------------------------------------------------------------------------- *)
 (** The [pure] judgement *)
 
